Work on CCP proof

proof/CCP/Coercion.v
@@ -2,92 +2,385 @@ Require Import Termes.
 Require Import Reduction.
 Require Import Conv.
 Require Import LiftSubst.
+Require Import Env.
 Require Import CCP.Types.
+Require Import CCP.Thinning.
+Require Import CCP.Substitution.
 
-Lemma refl_coerce : forall U, U >> U.
-Proof.
-  intros.
-  apply coerce_conv ; auto with coc core.
-Qed.
 
-Lemma coerce_conv_coerce : forall U U' V V', conv U U' -> conv V V' ->
-  U >> V -> U' >> V'.
-Proof.
+Inductive coerce_in_env : env -> env -> Prop :=
+| coerce_env_hd : forall e t u,
+  forall s, e |- t : (Srt s) -> e |- u : (Srt s) ->
+  e |- t >> u -> coerce_in_env (u :: e) (t :: e)
+| coerce_env_tl :
+        forall e f t, wf (t :: f) -> coerce_in_env e f -> coerce_in_env (t :: e) (t :: f).
+
+  Hint Resolve coerce_env_hd coerce_env_tl: coc.
+
+  Lemma conv_item :
+   forall n t e,
+   item_lift t e n ->
+   forall f, coerce_in_env e f ->
+   item_lift t f n \/
+   ((forall g, trunc _ (S n) e g -> trunc _ (S n) f g) /\
+   exists u, item_lift u f n /\ (ex2 (fun s => f |- u : (Srt s)) (fun s => f |- t : Srt s) /\
+   (wf f -> f |- u >> t))).
+simple induction n.
+do 3 intro.
+elim H.
+do 4 intro.
+rewrite H0.
+inversion_clear H1.
 intros.
-induction H1 ; auto with coc core.
-apply coerce_conv.
-apply trans_conv_conv with A ; auto with coc.
-apply trans_conv_conv with B ; auto with coc.
+inversion_clear H1.
+right.
+split; intros.
+inversion_clear H1; auto with coc core arith datatypes.
 
-apply coerce_trans with (Prod A' B') ; auto with coc core.
-apply coerce_trans with (Prod A B) ; auto with coc core.
-
-apply coerce_trans with (Sum A' B') ; auto with coc core.
-apply coerce_trans with (Sum A B) ; auto with coc core.
-
-apply coerce_trans with (Subset U P) ; auto with coc core.
-apply coerce_sub_l ; auto with coc core.
-apply coerce_trans with U'0 ; auto with coc core.
-
-apply coerce_trans with (Subset U'0 P) ; auto with coc core.
-apply coerce_sub_r ; auto with coc core.
-apply coerce_trans with U ; auto with coc core.
-
-apply coerce_trans with A ; auto with coc core.
-apply coerce_trans with B ; auto with coc core.
-apply coerce_trans with C ; auto with coc core.
-Qed.
-
-Lemma sym_coerce : forall U V, U >> V -> V >> U.
-Proof.
+exists (lift 1 t0).
 intros.
-induction H ; auto with coc.
+split.
+inversion_clear H.
 
-apply coerce_trans with B ; auto with coc.
+exists t0; auto with coc core arith datatypes.
+
+split.
+exists s ; auto with coc core.
+change (Srt s) with (lift 1 (Srt s)). 
+apply thinning_n with l ; auto with coc core.
+apply wf_var with s ; auto with coc.
+
+change (Srt s) with (lift 1 (Srt s)). 
+apply thinning_n with l ; auto with coc core.
+apply wf_var with s ; auto with coc.
+apply thinning_n_coerce with l; auto with coc.
+
+left.
+exists x; auto with coc core arith datatypes.
+
+do 5 intro.
+elim H0.
+do 4 intro.
+rewrite H1.
+inversion_clear H2.
+intros.
+inversion_clear H2.
+left.
+exists x; auto with coc core arith datatypes.
+
+elim H with (lift (S n0) x) l f0; auto with coc core arith datatypes; intros.
+left.
+elim H2; intros.
+exists x0; auto with coc core arith datatypes.
+rewrite simpl_lift.
+pattern (lift (S (S n0)) x0) in |- *.
+rewrite simpl_lift.
+elim H6; auto with coc core arith datatypes.
+
+right.
+elim H2.
+clear H2.
+simple induction 2; intros.
+clear H6.
+split; intros.
+inversion_clear H6; auto with coc core arith datatypes.
+
+destruct H7.
+destruct H7.
+destruct H7.
+exists (lift 1 x0).
+split ; auto with coc core.
+inversion_clear H6 ; auto with coc core arith.
+exists x2.
+rewrite H10.
+rewrite <- simpl_lift.
+auto with coc core.
+auto with coc.
+
+split.
+exists x1 ; change (Srt x1) with (lift 1 (Srt x1)). 
+apply thinning_n with f0 ; auto with coc core.
+rewrite simpl_lift.
+apply thinning_n with f0 ; auto with coc core.
+
+intros.
+pattern (lift (S (S n0)) x).
+rewrite simpl_lift.
+apply thinning_n_coerce with f0 ; auto with coc arith datatypes.
+inversion_clear H6; auto.
+pose (typ_wf _ _ _ H7).
+apply (H8 w).
+
+exists x; auto with coc core arith datatypes.
 Qed.
 
-Lemma coerce_subst_rec : forall U V,  U >> V -> forall u v, conv u v -> forall n, subst_rec u U n >> subst_rec v V n.
-Proof.
-  induction 1 ; intros ; simpl.
-  apply coerce_conv ; auto with coc.
- 
- apply coerce_prod ; auto with coc.
+Lemma typ_conv_env :
+  forall e t T, typ e t T -> 
+  forall f, coerce_in_env e f -> 
+  wf f -> typ f t T.
+intros e t T IHt.
+induction IHt using typ_mut with 
+(P := fun e t T => fun H : typ e t T =>
+  forall f, coerce_in_env e f -> 
+  wf f -> typ f t T)
+(P0 := fun e T U => fun H : e |- T >> U =>
+  forall f, coerce_in_env e f -> 
+  wf f -> f |- T >> U) ; intros ;
+auto with coc core arith datatypes.
 
- apply coerce_sum ; auto with coc.
+elim conv_item with n T e f; auto with coc core arith datatypes; intros.
+repeat destruct H1.
+destruct H2.
+destruct H2.
+destruct H3.
+destruct H3.
+apply type_conv with x x0 ; auto with coc core.
 
- apply coerce_sub_l ; auto with coc.
+cut (wf (T :: f)); intros.
+apply type_abs with s1 s2; auto with coc core arith datatypes.
+apply wf_var with s1; auto with coc core arith datatypes.
 
- apply coerce_sub_r ; auto with coc.
+apply type_app with V; auto with coc core arith datatypes.
 
- apply coerce_trans with (subst_rec u B n) ; auto with coc.
+cut (wf (U :: f)); intros.
+apply type_pair with s1 s2; auto with coc core arith datatypes.
+apply wf_var with s1 ; auto with coc core.
+
+cut (wf (T :: f)); intros.
+apply type_prod with s1; auto with coc core arith datatypes.
+
+apply wf_var with s1; auto with coc core arith datatypes.
+
+cut (wf (T :: f)); intros.
+apply type_sum with s1; auto with coc core arith datatypes.
+
+apply wf_var with s1; auto with coc core arith datatypes.
+
+cut (wf (T :: f)); intros.
+apply type_subset; auto with coc core arith datatypes.
+
+apply wf_var with set; auto with coc core arith datatypes.
+
+apply type_pi1 with V ; auto with coc core arith datatypes.
+
+apply type_pi2 with U ; auto with coc core arith datatypes.
+
+cut (wf (U :: f)); intros.
+apply type_let_in with U s1 s2 ; auto with coc core arith datatypes.
+apply wf_var with s1 ; auto with coc core.
+
+apply type_conv with U s; auto with coc core arith datatypes.
+
+cut (wf (A' :: f)) ; intros.
+apply coerce_prod with s ;auto with coc core arith datatypes.
+apply wf_var with s ; auto with coc core arith datatypes.
+
+cut (wf (A :: f)) ; intros.
+apply coerce_sum with s ;auto with coc core arith datatypes.
+apply wf_var with s ; auto with coc core arith datatypes.
+
+apply coerce_beta with B C s ; auto with coc core arith datatypes.
 Qed.
 
-Lemma subst_coerce : forall U V, U >> V -> forall t, subst t U >> subst t V.
+Lemma coerce_conv_env :
+  forall e T U, e |- T >> U -> 
+  forall f, coerce_in_env e f -> 
+  wf f -> f |- T >> U.
+intros e t T IHc.
+induction IHc using coerce_mut with 
+(P := fun e t T => fun H : typ e t T =>
+  forall f, coerce_in_env e f -> 
+  wf f -> typ f t T)
+(P0 := fun e T U => fun H : e |- T >> U =>
+  forall f, coerce_in_env e f -> 
+  wf f -> f |- T >> U) ; intros ;
+auto with coc core arith datatypes.
+
+elim conv_item with n T e f; auto with coc core arith datatypes; intros.
+repeat destruct H1.
+destruct H2.
+destruct H2.
+destruct H3.
+destruct H3.
+apply type_conv with x x0 ; auto with coc core.
+
+cut (wf (T :: f)); intros.
+apply type_abs with s1 s2; auto with coc core arith datatypes.
+apply wf_var with s1; auto with coc core arith datatypes.
+
+apply type_app with V; auto with coc core arith datatypes.
+
+cut (wf (U :: f)); intros.
+apply type_pair with s1 s2; auto with coc core arith datatypes.
+apply wf_var with s1 ; auto with coc core.
+
+cut (wf (T :: f)); intros.
+apply type_prod with s1; auto with coc core arith datatypes.
+
+apply wf_var with s1; auto with coc core arith datatypes.
+
+cut (wf (T :: f)); intros.
+apply type_sum with s1; auto with coc core arith datatypes.
+
+apply wf_var with s1; auto with coc core arith datatypes.
+
+cut (wf (T :: f)); intros.
+apply type_subset; auto with coc core arith datatypes.
+
+apply wf_var with set; auto with coc core arith datatypes.
+
+apply type_pi1 with V ; auto with coc core arith datatypes.
+
+apply type_pi2 with U ; auto with coc core arith datatypes.
+
+cut (wf (U :: f)); intros.
+apply type_let_in with U s1 s2 ; auto with coc core arith datatypes.
+apply wf_var with s1 ; auto with coc core.
+
+apply type_conv with U s; auto with coc core arith datatypes.
+
+cut (wf (A' :: f)) ; intros.
+apply coerce_prod with s ;auto with coc core arith datatypes.
+apply wf_var with s ; auto with coc core arith datatypes.
+
+cut (wf (A :: f)) ; intros.
+apply coerce_sum with s ;auto with coc core arith datatypes.
+apply wf_var with s ; auto with coc core arith datatypes.
+
+apply coerce_beta with B C s ; auto with coc core arith datatypes.
+Qed.
+
+Lemma subset_support_not_sort : forall e t T, e |- t : T -> 
+  forall U P, t = Subset U P -> 
+  forall s, ~ (conv U (Srt s)).
 Proof.
+  induction 1 ; intros ; try discriminate.
+
+  red ; intros.
+  injection H1.
   intros.
-  unfold subst ; apply coerce_subst_rec ; auto with coc.
-Qed.
+  rewrite <- H4 in H2.
+Admitted.
 
-Lemma coerce_lift_rec : forall U V,  U >> V -> forall n k, lift_rec k U n >> lift_rec k V n.
+Require Import CCP.Generation.
+
+Lemma coerce_sort : forall e T U, e |- T >> U ->
+  forall r, e |- T : (Srt r) -> e |- U : (Srt r) ->
+  forall s,
+  (conv T (Srt s) -> conv U (Srt s)) /\ (conv U (Srt s) -> conv T (Srt s)).
 Proof.
-  induction 1 ; intros ; simpl.
-  apply coerce_conv ; auto with coc.
- 
- apply coerce_prod ; auto with coc.
+  induction 1
+ using coerce_mut with
+  (P := fun e t T => fun H : typ e t T =>
+  forall s, T = (Srt s) ->
+  forall T', e |- t : T' -> T' = (Srt s))
+(P0 := fun e T U => fun H : e |- T >> U =>
+  forall r, e |- T : (Srt r) -> e |- U : (Srt r) ->
+  forall s,
+  (conv T (Srt s) -> conv U (Srt s)) /\ (conv U (Srt s) -> conv T (Srt s))) ; intros ;
+auto with coc core arith datatypes ; try discriminate.
 
- apply coerce_sum ; auto with coc.
-
- apply coerce_sub_l ; auto with coc.
-
- apply coerce_sub_r ; auto with coc.
-
- apply coerce_trans with (lift_rec k B n) ; auto with coc.
-Qed.
-
-Lemma lift_coerce : forall U V, U >> V -> forall n, lift n U >> lift n V.
-Proof.
+  injection H.
   intros.
-  unfold lift ; apply coerce_lift_rec ; auto with coc.
-Qed.
+  inversion H0.
+  rewrite H1 ; auto.
 
-Hint Resolve refl_coerce sym_coerce subst_coerce lift_coerce : coc.
+  destruct (typ_sort H2 (refl_equal (Srt prop))).
+  rewrite H10 in H4.
+  pose (typ_not_kind H4).
+  elim n ; auto.
+
+  injection H.
+  intros.
+  case (typ_sort H0 (refl_equal (Srt set))).
+  intros.
+  rewrite <- H1.
+  auto with coc.
+  
+  inversion i.
+
+
+  induction H0.
+
+  
+  Focus 3.
+
+  ssplit ; auto with coc.
+  pose (type_subset _ _ t _ t0).
+  injection H ; intros.
+  rewrite <- H1.
+  apply (subset_support_not_sort _ _ _ t1 T U (refl_equal (Subset T U)) s).
+
+  pose (IHcoerce2 s t2 t1).
+  pose (IHcoerce U0 P H0).
+  destruct a0.
+  destruct (a set).
+  split.
+  apply (H3 H1).
+  assumption.
+
+  intuition.
+  
+  elim (conv_sort_prod s0 A B) ; auto with coc core.
+  elim (conv_sort_prod s0 A' B') ; auto with coc core.
+
+  intuition.
+  
+  elim (conv_sort_sum s0 A B) ; auto with coc core.
+  elim (conv_sort_sum s0 A' B') ; auto with coc core.
+
+  intuition.
+  
+  elim (conv_sort_subset s U P) ; auto with coc core.
+
+  pose (subset_support_not_sort _ _ _ H0 U P (refl_equal (Subset U P)) s).
+
+  inversion H0.
+  rewrite <- H6 in H1.
+  induction (IHcoerce _ H7 H1 s).
+  pose (H10 H2).
+
+  pose (subset_support_not_sort _ _ _ H0 U P (refl_equal (Subset U P)) s).
+  contradiction.
+
+
+  
+  
+
+  
+  
+
+  elim (conv_sort_prod s U P) ; auto with coc core.
+
+
+
+
+Lemma coerce_sym : forall e T U, e |- T >> U ->
+  forall s, e |- T : Srt s -> e |- U : Srt s -> 
+  e |- U >> T.
+Proof.
+  intros e T U H ; induction H ; intros ; auto with coc core.
+  
+  apply coerce_prod with s ; auto with coc.
+  apply IHcoerce1 with s ; auto with coc. 
+  
+  cut (coerce_in_env (A' :: G) (A :: G)).
+  cut (coerce_in_env (A :: G) (A' :: G)).
+  intros.
+  
+  apply coerce_conv_env with (A' :: G) ; auto with coc core.
+ 
+  inversion_clear H3.
+  apply IHcoerce2 with s0 ; auto with coc.
+  
+  apply typ_conv_env with (A :: G) ; auto with coc core.
+  apply wf_var with s ; auto with coc core.
+  
+  inversion_clear H4 ; auto with coc core.
+  inversion H11.
+  apply typ_conv_env with (A :: G) ; auto with coc core.
+  apply wf_var with s ; auto with coc core.
+
+  apply coerce_env_
+
+  
