proof/CCP/Inversion.v
@@ -5,6 +5,8 @@ Require Import LiftSubst.
 Require Import Env.
 Require Import CCP.Types.
 Require Import CCP.Coercion.
+Require Import CCP.Thinning.
+Require Import CCP.Substitution.
 
 Implicit Types i k m n p : nat.
 Implicit Type s : sort.
@@ -13,52 +15,55 @@ Implicit Types e f g : env.
 
   Definition inv_type (P : Prop) e t T : Prop :=
     match t with
-    | Srt prop => coerce T (Srt kind) -> P
-    | Srt set => coerce T (Srt kind) -> P
+    | Srt prop => coerce e T (Srt kind) -> P
+    | Srt set => coerce e T (Srt kind) -> P
     | Srt kind => True
-    | Ref n => forall x : term, item _ x e n -> coerce T (lift (S n) x) -> P
+    | Ref n => forall x : term, item _ x e n -> coerce e T (lift (S n) x) -> P
     | Abs A M =>
         forall s1 s2 (U : term),
         typ e A (Srt s1) ->
-        typ (A :: e) M U -> typ (A :: e) U (Srt s2) -> coerce T (Prod A U) -> P
+        typ (A :: e) M U -> typ (A :: e) U (Srt s2) -> coerce e T (Prod A U) -> P
     | App u v =>
         forall Ur V : term,
-        typ e v V -> typ e u (Prod V Ur) -> coerce T (subst v Ur) -> P
+        typ e v V -> typ e u (Prod V Ur) -> coerce e T (subst v Ur) -> P
     | Pair T' u v => 
         forall U s1, typ e U (Srt s1) ->
 	  typ e u U -> 
 	  forall V s2, typ (U :: e) V (Srt s2) ->
-            typ e v (subst u V) -> T' = (Sum U V) -> coerce T (Sum U V) -> P
+            typ e v (subst u V) -> T' = (Sum U V) -> coerce e T (Sum U V) -> P
     | Prod A B =>
         forall s1 s2,
-        typ e A (Srt s1) -> typ (A :: e) B (Srt s2) -> coerce T (Srt s2) -> P
+        typ e A (Srt s1) -> typ (A :: e) B (Srt s2) -> coerce e T (Srt s2) -> P
     | Sum A B =>
         forall s1 s2,
-        typ e A (Srt s1) -> typ (A :: e) B (Srt s2) -> coerce T (Srt s2) -> P
+        typ e A (Srt s1) -> typ (A :: e) B (Srt s2) -> coerce e T (Srt s2) -> P
     | Subset A B =>
-        typ e A (Srt set) -> typ (A :: e) B (Srt prop) -> coerce T (Srt set) -> P
+        typ e A (Srt set) -> typ (A :: e) B (Srt prop) -> coerce e T (Srt set) -> P
     | Pi1 t =>
         forall U V,
-        typ e t (Sum U V) -> coerce T U -> P
+        typ e t (Sum U V) -> coerce e T U -> P
     | Pi2 t =>
         forall U V,
-        typ e t (Sum U V) -> coerce T (subst (Pi1 t) V) -> P
+        typ e t (Sum U V) -> coerce e T (subst (Pi1 t) V) -> P
     | Let_in t v =>
         forall U, typ e t U -> 
 	forall s1, typ e U (Srt s1) ->
         forall M, typ (U :: e) v M -> 
         forall s2, typ (U :: e) M (Srt s2) ->
-        coerce T (subst t M) -> P
+        coerce e T (subst t M) -> P
     end.
+    
+
 
   Lemma inv_type_coerce :
    forall (P : Prop) e t (U V : term),
-   coerce U V -> inv_type P e t U -> inv_type P e t V.
-do 6 intro.
-cut (forall x : term, coerce V x -> coerce U x).
+   forall s, e |- U : (Srt s) -> e |- V : (Srt s) ->
+   coerce e V U -> inv_type P e t U -> inv_type P e t V.
+intros P e t U V UVs Us Vs.
 intro.
+
 case t; simpl in |- *; intros.
-generalize H1 ; clear H1.
+generalize H0 ; clear H0.
 elim s; auto with coc core arith datatypes; intros.
 
 apply H1 with x; auto with coc core arith datatypes.
@@ -80,9 +85,13 @@ apply H1 with U0 V0; auto with coc core arith datatypes.
 apply H1 with U0 s1 M s2; auto with coc core arith datatypes.
 
 intros.
+induction H ; induction H0 ; auto with coc core.
+
+Admitted.
+(*pose coerce_beta.
 apply coerce_trans with V; auto with coc core arith datatypes.
 Qed.
-
+*)
   Theorem typ_inversion :
    forall (P : Prop) e t T, typ e t T -> inv_type P e t T -> P.
 simple induction 1; simpl in |- *; intros.
@@ -110,7 +119,7 @@ apply H2 with U V; auto with coc core arith datatypes.
 apply H8 with U s1 M s2; auto with coc core arith datatypes.
 
 apply H1.
-apply inv_type_coerce with V; auto with coc core arith datatypes.
+apply inv_type_coerce with V s; auto with coc core arith datatypes.
 Qed.
 
 
@@ -120,13 +129,13 @@ apply typ_inversion with e (Srt kind) t; simpl in |- *;
  auto with coc core arith datatypes.
 Qed.
 
-  Lemma inv_typ_prop : forall e T, typ e (Srt prop) T -> coerce T (Srt kind).
+  Lemma inv_typ_prop : forall e T, typ e (Srt prop) T -> coerce e T (Srt kind).
 intros.
 apply typ_inversion with e (Srt prop) T; simpl in |- *;
  auto with coc core arith datatypes.
 Qed.
 
-  Lemma inv_typ_set : forall e T, typ e (Srt set) T -> coerce T (Srt kind).
+  Lemma inv_typ_set : forall e T, typ e (Srt set) T -> coerce e T (Srt kind).
 intros.
 apply typ_inversion with e (Srt set) T; simpl in |- *;
  auto with coc core arith datatypes.
@@ -135,7 +144,7 @@ Qed.
   Lemma inv_typ_ref :
    forall (P : Prop) e T n,
    typ e (Ref n) T ->
-   (forall U : term, item _ U e n -> coerce T (lift (S n) U) -> P) -> P.
+   (forall U : term, item _ U e n -> coerce e T (lift (S n) U) -> P) -> P.
 intros.
 apply typ_inversion with e (Ref n) T; simpl in |- *; intros;
  auto with coc core arith datatypes.
@@ -147,7 +156,7 @@ Qed.
    typ e (Abs A M) U ->
    (forall s1 s2 T,
     typ e A (Srt s1) ->
-    typ (A :: e) M T -> typ (A :: e) T (Srt s2) -> coerce (Prod A T) U -> P) ->
+    typ (A :: e) M T -> typ (A :: e) T (Srt s2) -> coerce e (Prod A T) U -> P) ->
    P.
 intros.
 apply typ_inversion with e (Abs A M) U; simpl in |- *;
@@ -159,7 +168,7 @@ Qed.
    forall (P : Prop) e u v T,
    typ e (App u v) T ->
    (forall V Ur : term,
-    typ e u (Prod V Ur) -> typ e v V -> coerce T (subst v Ur) -> P) -> P.
+    typ e u (Prod V Ur) -> typ e v V -> coerce e T (subst v Ur) -> P) -> P.
 intros.
 apply typ_inversion with e (App u v) T; simpl in |- *;
  auto with coc core arith datatypes; intros.
@@ -172,7 +181,7 @@ Qed.
    (forall T U V : term, forall s1 s2,
      typ e U (Srt s1) ->
      typ e u U -> typ (U :: e) V (Srt s2) -> typ e v (subst u V) ->
-     T = (Sum U V) -> coerce T' (Sum U V) -> P) -> P.
+     T = (Sum U V) -> coerce e T' (Sum U V) -> P) -> P.
 intros.
 apply typ_inversion with e (Pair T u v) T'; simpl in |- *;
  auto with coc core arith datatypes; intros.
@@ -183,7 +192,7 @@ Qed.
    forall (P : Prop) e T (U s : term),
    typ e (Prod T U) s ->
    (forall s1 s2,
-    typ e T (Srt s1) -> typ (T :: e) U (Srt s2) -> coerce (Srt s2) s -> P) -> P.
+    typ e T (Srt s1) -> typ (T :: e) U (Srt s2) -> coerce e (Srt s2) s -> P) -> P.
 intros.
 apply typ_inversion with e (Prod T U) s; simpl in |- *;
  auto with coc core arith datatypes; intros.
@@ -194,7 +203,7 @@ Qed.
    forall (P : Prop) e T (U s : term),
    typ e (Sum T U) s ->
    (forall s1 s2,
-    typ e T (Srt s1) -> typ (T :: e) U (Srt s2) -> coerce (Srt s2) s -> P) -> P.
+    typ e T (Srt s1) -> typ (T :: e) U (Srt s2) -> coerce e (Srt s2) s -> P) -> P.
 intros.
 apply typ_inversion with e (Sum T U) s; simpl in |- *;
  auto with coc core arith datatypes; intros.
@@ -204,7 +213,7 @@ Qed.
   Lemma inv_typ_subset :
    forall (P : Prop) e T (U s : term),
    typ e (Subset T U) s ->
-   (typ e T (Srt set) -> typ (T :: e) U (Srt prop) -> coerce (Srt set) s -> P) -> P.
+   (typ e T (Srt set) -> typ (T :: e) U (Srt prop) -> coerce e (Srt set) s -> P) -> P.
 intros.
 apply typ_inversion with e (Subset T U) s; simpl in |- *;
  auto with coc core arith datatypes; intros.
@@ -213,7 +222,7 @@ Qed.
 Lemma inv_typ_pi1 : 
   forall (P : Prop) e t T,
    typ e (Pi1 t) T ->
-   (forall U V, typ e t (Sum U V) ->  coerce U T -> P) -> P.
+   (forall U V, typ e t (Sum U V) ->  coerce e U T -> P) -> P.
 Proof.
 intros.
 apply typ_inversion with e (Pi1 t) T; simpl in |- *;
@@ -224,7 +233,7 @@ Qed.
 Lemma inv_typ_pi2 : 
   forall (P : Prop) e t T,
    typ e (Pi2 t) T ->
-   (forall U V, typ e t (Sum U V) ->  coerce (subst (Pi1 t) V) T -> P) -> P.
+   (forall U V, typ e t (Sum U V) ->  coerce e (subst (Pi1 t) V) T -> P) -> P.
 Proof.
 intros.
 apply typ_inversion with e (Pi2 t) T; simpl in |- *;
@@ -239,7 +248,7 @@ Lemma inv_typ_let_in :
    forall s1, typ e V (Srt s1) ->
    forall T', typ (V :: e) t T' ->
    forall s2, typ (V :: e) T' (Srt s2) ->
-   coerce (subst v T')  T -> P) -> P.
+   coerce e (subst v T')  T -> P) -> P.
 Proof.
 intros.
 apply typ_inversion with e (Let_in v t) T; simpl in |- *;
@@ -304,7 +313,7 @@ inversion_clear H2.
 Qed.
 
 Lemma type_pair_unique : forall e t T, typ e t T -> forall U V u v, t = (Pair (Sum U V) u v) ->
-   coerce T (Sum U V).
+   coerce e T (Sum U V).
 Proof.
 intros ; induction H ; try discriminate.
 injection H0 ; intros.
@@ -316,7 +325,7 @@ Qed.
 
 Lemma type_pair_unique2 : forall e t T, typ e t T -> 
    forall T' u v, t = (Pair T' u v) -> exists U,  exists  V, T' = Sum U V /\ 
-   coerce T (Sum U V).
+   coerce e T (Sum U V).
 Proof.
 intros ; induction H ; try discriminate.
 injection H0 ; intros.
