proof/CCP/Substitution.v
@@ -3,8 +3,6 @@ Require Import Reduction.
 Require Import LiftSubst.
 Require Import Env.
 Require Import CCP.Types.
-Require Import CCP.Coercion.
-Require Import CCP.Inversion.
 Require Import CCP.Thinning.
 
 Implicit Types i k m n p : nat.
@@ -12,41 +10,6 @@ Implicit Type s : sort.
 Implicit Types A B M N T t u v : term.
 Implicit Types e f g : env.
 
-  Lemma wf_sort_lift :
-   forall n e t, wf e -> item_lift t e n -> exists s : sort, typ e t (Srt s).
-simple induction n.
-simple destruct e; intros.
-elim H0; intros.
-inversion_clear H2.
-
-elim H0; intros.
-rewrite H1.
-inversion_clear H2.
-inversion_clear H.
-exists s.
-replace (Srt s) with (lift 1 (Srt s)); auto with coc core arith datatypes.
-apply thinning; auto with coc core arith datatypes.
-apply wf_var with s; auto with coc core arith datatypes.
-
-intros.
-elim H1; intros.
-rewrite H2.
-generalize H0.
-inversion_clear H3; intros.
-rewrite simpl_lift; auto with coc core arith datatypes.
-cut (wf l); intros.
-elim H with l (lift (S n0) x); intros; auto with coc core arith datatypes.
-inversion_clear H3.
-exists x0.
-change (typ (y :: l) (lift 1 (lift (S n0) x)) (lift 1 (Srt x0))) in |- *.
-apply thinning; auto with coc core arith datatypes.
-apply wf_var with s; auto with coc core arith datatypes.
-
-exists x; auto with coc core arith datatypes.
-
-inversion_clear H3.
-apply typ_wf with y (Srt s); auto with coc core arith datatypes.
-Qed.
 
   Lemma typ_sub_weak :
    forall g (d : term) t,
@@ -56,33 +19,51 @@ Qed.
    forall f n,
    sub_in_env d t n e f ->
    wf f -> trunc _ n f g -> typ f (subst_rec d u n) (subst_rec d U n).
-simple induction 2; simpl in |- *; intros; auto with coc core arith datatypes.
-elim (lt_eq_lt_dec n v); [ intro Hlt_eq | intro Hlt ].
-elim H2.
+intros g d t H.
+intros e u U H0.
+induction H0 using typ_mut with
+ (P := fun e u (U : term) => fun H0 : e |- u : U =>
+ forall f n,
+ sub_in_env d t n e f ->
+ wf f -> trunc term n f g -> f |- subst_rec d u n : subst_rec d U n)
+ (P0 :=
+ fun e T (U : term) => fun H0 : e |- T >> U =>
+ forall f n,
+ sub_in_env d t n e f ->
+ wf f -> trunc term n f g -> f |- subst_rec d T n >> subst_rec d U n) ;
+ simpl in |- *;
+ try simpl in IHtyp ; 
+ try simpl in IHtyp1 ;
+ try simpl in IHtyp2 ;
+ try simpl in IHtyp3 ; 
+ try simpl in IHtyp4 ; intros; auto with coc core arith datatypes.
+
+elim (lt_eq_lt_dec n0 n); [ intro Hlt_eq | intro Hlt ].
+elim i.
 elim Hlt_eq; clear Hlt_eq.
-case v; [ intro Hlt | intros n0 Hlt ]; intros.
+case n; [ intro Hlt | intros n1 Hlt ]; intros.
 inversion_clear Hlt.
 
 simpl in |- *.
-rewrite H6.
+rewrite H3.
 rewrite simpl_subst; auto with coc core arith datatypes.
 apply type_var; auto with coc core arith datatypes.
 exists x; auto with coc core arith datatypes.
-apply nth_sub_sup with d t n e0; auto with coc core arith datatypes.
+apply nth_sub_sup with d t n0 e; auto with coc core arith datatypes.
 
 intro Heq; intros.
-rewrite H6.
+rewrite H3.
 elim Heq.
 rewrite simpl_subst; auto with coc core arith datatypes.
 replace x with t.
 apply thinning_n with g; auto with coc core arith datatypes.
 
-apply fun_item with e0 v; auto with coc core arith datatypes.
+apply fun_item with e n; auto with coc core arith datatypes.
 apply nth_sub_eq with d f; auto with coc core arith datatypes.
 elim Heq; auto with coc core arith datatypes.
 
 apply type_var; auto with coc core arith datatypes.
-apply nth_sub_inf with t e0; auto with coc core arith datatypes.
+apply nth_sub_inf with t e; auto with coc core arith datatypes.
 
 cut (wf (subst_rec d T n :: f)); intros.
 apply type_abs with s1 s2; auto with coc core arith datatypes.
@@ -93,7 +74,7 @@ rewrite distr_subst.
 apply type_app with (subst_rec d V n); auto with coc core arith datatypes.
 
 apply type_pair with s1 s2 ; auto with coc core arith datatypes.
-apply H6 ; auto with coc.
+apply IHtyp3 ; auto with coc.
 apply wf_var with s1 ; auto with coc.
 rewrite <- distr_subst ; auto with coc core arith datatypes.
 
@@ -116,15 +97,135 @@ apply type_pi1 with (subst_rec d V (S n)) ; auto with coc.
 
 rewrite distr_subst.
 simpl.
-apply type_pi2 with (subst_rec d U0 n) ; auto with coc.
+apply type_pi2 with (subst_rec d U n) ; auto with coc.
 
-cut (wf (subst_rec d U0 n :: f)).
+cut (wf (subst_rec d U n :: f)).
 intro ; rewrite distr_subst.
-apply type_let_in with (subst_rec d U0 n) s1 s2 ; auto with coc core arith datatypes.
+apply type_let_in with (subst_rec d U n) s1 s2 ; auto with coc core arith datatypes.
 apply wf_var with s1 ; auto with coc core arith datatypes.
 
-apply type_conv with (subst_rec d U0 n) s; auto with coc core arith datatypes.
-apply coerce_subst_rec ; auto with coc core.
+apply type_conv with (subst_rec d U n) s; auto with coc core arith datatypes.
+
+apply coerce_prod with s ; auto with coc core.
+
+apply IHtyp4 ; auto with coc core.
+apply wf_var with s ; auto with coc core.
+
+apply coerce_sum with s ; auto with coc core.
+
+apply IHtyp4 ; auto with coc core.
+apply wf_var with s ; auto with coc core.
+
+apply coerce_beta with (subst_rec d B n) (subst_rec d C n) s ; auto with coc core.
+Qed.
+
+Lemma coerce_sub_weak :
+   forall g (d : term) t,
+   typ g d t ->
+   forall e T (U : term),
+   e |- T >> U ->
+   forall f n,
+   sub_in_env d t n e f ->
+   wf f -> trunc _ n f g -> f |- (subst_rec d T n) >> (subst_rec d U n).
+intros g d t H.
+intros e u U H0.
+induction H0 using coerce_mut with
+ (P := fun e u (U : term) => fun H0 : e |- u : U =>
+ forall f n,
+ sub_in_env d t n e f ->
+ wf f -> trunc term n f g -> f |- subst_rec d u n : subst_rec d U n)
+ (P0 :=
+ fun e T (U : term) => fun H0 : e |- T >> U =>
+ forall f n,
+ sub_in_env d t n e f ->
+ wf f -> trunc term n f g -> f |- subst_rec d T n >> subst_rec d U n) ;
+ simpl in |- *;
+ try simpl in IHcoerce ; 
+ try simpl in IHcoerce0 ; 
+ try simpl in IHcoerce1 ;
+ try simpl in IHcoerce2 ;
+ try simpl in IHcoerce3 ; 
+ try simpl in IHcoerce4 ; intros; auto with coc core arith datatypes.
+
+elim (lt_eq_lt_dec n0 n); [ intro Hlt_eq | intro Hlt ].
+elim i.
+elim Hlt_eq; clear Hlt_eq.
+case n; [ intro Hlt | intros n1 Hlt ]; intros.
+inversion_clear Hlt.
+
+simpl in |- *.
+rewrite H3.
+rewrite simpl_subst; auto with coc core arith datatypes.
+apply type_var; auto with coc core arith datatypes.
+exists x; auto with coc core arith datatypes.
+apply nth_sub_sup with d t n0 e; auto with coc core arith datatypes.
+
+intro Heq; intros.
+rewrite H3.
+elim Heq.
+rewrite simpl_subst; auto with coc core arith datatypes.
+replace x with t.
+apply thinning_n with g; auto with coc core arith datatypes.
+
+apply fun_item with e n; auto with coc core arith datatypes.
+apply nth_sub_eq with d f; auto with coc core arith datatypes.
+elim Heq; auto with coc core arith datatypes.
+
+apply type_var; auto with coc core arith datatypes.
+apply nth_sub_inf with t e; auto with coc core arith datatypes.
+
+cut (wf (subst_rec d T n :: f)); intros.
+apply type_abs with s1 s2; auto with coc core arith datatypes.
+
+apply wf_var with s1; auto with coc core arith datatypes.
+
+rewrite distr_subst.
+apply type_app with (subst_rec d V n); auto with coc core arith datatypes.
+
+apply type_pair with s1 s2 ; auto with coc core arith datatypes.
+apply IHcoerce1 ; auto with coc.
+apply wf_var with s1 ; auto with coc.
+rewrite <- distr_subst ; auto with coc core arith datatypes.
+
+cut (wf (subst_rec d T n :: f)); intros.
+apply type_prod with s1; auto with coc core arith datatypes.
+
+apply wf_var with s1; auto with coc core arith datatypes.
+
+cut (wf (subst_rec d T n :: f)); intros.
+apply type_sum with s1; auto with coc core arith datatypes.
+
+apply wf_var with s1; auto with coc core arith datatypes.
+
+cut (wf (subst_rec d T n :: f)); intros.
+apply type_subset; auto with coc core arith datatypes.
+
+apply wf_var with set; auto with coc core arith datatypes.
+
+apply type_pi1 with (subst_rec d V (S n)) ; auto with coc.
+
+rewrite distr_subst.
+simpl.
+apply type_pi2 with (subst_rec d U n) ; auto with coc.
+
+cut (wf (subst_rec d U n :: f)).
+intro ; rewrite distr_subst.
+apply type_let_in with (subst_rec d U n) s1 s2 ; auto with coc core arith datatypes.
+apply wf_var with s1 ; auto with coc core arith datatypes.
+
+apply type_conv with (subst_rec d U n) s; auto with coc core arith datatypes.
+
+apply coerce_prod with s ; auto with coc core.
+
+apply IHcoerce4 ; auto with coc core.
+apply wf_var with s ; auto with coc core.
+
+apply coerce_sum with s ; auto with coc core.
+
+apply IHcoerce4 ; auto with coc core.
+apply wf_var with s ; auto with coc core.
+
+apply coerce_beta with (subst_rec d B n) (subst_rec d C n) s ; auto with coc core.
 Qed.
 
   Theorem substitution :
@@ -136,3 +237,16 @@ unfold subst in |- *.
 apply typ_sub_weak with e t (t :: e); auto with coc core arith datatypes.
 apply typ_wf with d t; auto with coc core arith datatypes.
 Qed.
+
+  Theorem substitution_coerce :
+   forall e t T (U : term),
+   (t :: e) |- T >> U ->
+   forall d : term, e |- d : t -> e |- (subst d T) >> (subst d U).
+intros.
+unfold subst in |- *.
+apply coerce_sub_weak with e t (t :: e); auto with coc core arith datatypes.
+apply typ_wf with d t; auto with coc core arith datatypes.
+Qed.
+
+Hint Resolve substitution substitution_coerce : coc.
+
