proof/CCP/Thinning.v
@@ -3,8 +3,6 @@ Require Import Reduction.
 Require Import LiftSubst.
 Require Import Env.
 Require Import CCP.Types.
-Require Import CCP.Coercion.
-Require Import CCP.Inversion.
 
 Implicit Types i k m n p : nat.
 Implicit Type s : sort.
@@ -16,20 +14,30 @@ Implicit Types e f g : env.
    typ e t T ->
    forall n f,
    ins_in_env A n e f -> wf f -> typ f (lift_rec 1 t n) (lift_rec 1 T n).
-simple induction 1; simpl in |- *; intros; auto with coc core arith datatypes.
-elim (le_gt_dec n v); intros; apply type_var;
+intros A e t T IHt.
+induction IHt using typ_mut with 
+ (P := fun e t T => fun IHt : typ e t T =>
+   forall n f,
+   ins_in_env A n e f -> wf f -> typ f (lift_rec 1 t n) (lift_rec 1 T n))
+ (P0 := fun e T U => fun IHt : coerce e T U =>
+   forall n f,
+   ins_in_env A n e f -> wf f -> coerce f (lift_rec 1 T n) (lift_rec 1 U n)) ;
+simpl in |- *; try simpl in IHIHt ; try simpl in IHIHt1 ; try simpl in IHIHt2 ; try simpl in IHIHt3 ; 
+try simpl in IHIHt4 ; intros; auto with coc core arith datatypes.
+
+elim (le_gt_dec n0 n); intros; apply type_var;
  auto with coc core arith datatypes.
-elim H1; intros.
+elim i; intros.
 exists x.
-rewrite H4.
+rewrite H1.
 unfold lift in |- *.
 rewrite simpl_lift_rec; simpl in |- *; auto with coc core arith datatypes.
 
-apply ins_item_ge with A n e0; auto with coc core arith datatypes.
+apply ins_item_ge with A n0 e; auto with coc core arith datatypes.
 
-apply ins_item_lt with A e0; auto with coc core arith datatypes.
+apply ins_item_lt with A e; auto with coc core arith datatypes.
 
-cut (wf (lift_rec 1 T0 n :: f)).
+cut (wf (lift_rec 1 T n :: f)).
 intro.
 apply type_abs with s1 s2 ; auto with coc core arith datatypes.
 apply wf_var with s1 ; auto with coc core arith datatypes.
@@ -38,24 +46,23 @@ rewrite distr_lift_subst.
 apply type_app with (lift_rec 1 V n); auto with coc core arith datatypes.
 
 apply type_pair with s1 s2 ; auto with coc core arith datatypes.
-apply H5 ; auto with coc core arith datatypes.
+apply IHIHt3 ; auto with coc core arith datatypes.
 apply wf_var with s1 ; auto with coc core arith datatypes.
 
 rewrite <- distr_lift_subst.
-apply H7 ; auto with coc core arith datatypes.
+apply IHIHt4 ; auto with coc core arith datatypes.
 
-cut (wf (lift_rec 1 T0 n :: f)).
+cut (wf (lift_rec 1 T n :: f)).
 intro.
 apply type_prod with s1; auto with coc core arith datatypes.
 apply wf_var with s1; auto with coc core arith datatypes.
 
-
-cut (wf (lift_rec 1 T0 n :: f)).
+cut (wf (lift_rec 1 T n :: f)).
 intro.
 apply type_sum with s1; auto with coc core arith datatypes.
 apply wf_var with s1; auto with coc core arith datatypes.
 
-cut (wf (lift_rec 1 T0 n :: f)).
+cut (wf (lift_rec 1 T n :: f)).
 intro.
 apply type_subset ; auto with coc core arith datatypes.
 apply wf_var with set; auto with coc core arith datatypes.
@@ -73,7 +80,103 @@ apply type_let_in with (lift_rec 1 U n) s1 s2 ; auto with coc core.
 apply wf_var with s1 ; auto with coc core.
 
 apply type_conv with (lift_rec 1 U n) s; auto with coc core arith datatypes.
-apply coerce_lift_rec ; auto with coc.
+
+apply coerce_prod with s ; auto with coc.
+apply IHIHt4; auto with coc.
+apply wf_var with s.
+apply IHIHt1 ; auto with coc core.
+
+apply coerce_sum with s ; auto with coc.
+apply IHIHt4; auto with coc.
+apply wf_var with s.
+apply IHIHt2 ; auto with coc core.
+
+apply coerce_beta with (lift_rec 1 B n) (lift_rec 1 C n) s ; auto with coc core.
+Qed.
+
+  Lemma coerce_weak_weak :
+   forall A e T U,
+   e |- T >> U ->
+   forall n f,
+   ins_in_env A n e f -> wf f -> coerce f (lift_rec 1 T n) (lift_rec 1 U n).
+intros A e t T IHc.
+induction IHc using coerce_mut with 
+ (P := fun e t T => fun IHt : typ e t T =>
+   forall n f,
+   ins_in_env A n e f -> wf f -> typ f (lift_rec 1 t n) (lift_rec 1 T n))
+ (P0 := fun e T U => fun IHt : coerce e T U =>
+   forall n f,
+   ins_in_env A n e f -> wf f -> coerce f (lift_rec 1 T n) (lift_rec 1 U n)) ;
+simpl in |- *; try simpl in IHIHc ; try simpl in IHIHc0 ; try simpl in IHIHc1 ; try simpl in IHIHc2 ; try simpl in IHIHc3 ; 
+try simpl in IHIHc4 ; intros; auto with coc core arith datatypes.
+
+elim (le_gt_dec n0 n); intros; apply type_var;
+ auto with coc core arith datatypes.
+elim i; intros.
+exists x.
+rewrite H1.
+unfold lift in |- *.
+rewrite simpl_lift_rec; simpl in |- *; auto with coc core arith datatypes.
+
+apply ins_item_ge with A n0 e; auto with coc core arith datatypes.
+
+apply ins_item_lt with A e; auto with coc core arith datatypes.
+
+cut (wf (lift_rec 1 T n :: f)).
+intro.
+apply type_abs with s1 s2 ; auto with coc core arith datatypes.
+apply wf_var with s1 ; auto with coc core arith datatypes.
+
+rewrite distr_lift_subst.
+apply type_app with (lift_rec 1 V n); auto with coc core arith datatypes.
+
+apply type_pair with s1 s2 ; auto with coc core arith datatypes.
+apply IHIHc1 ; auto with coc core arith datatypes.
+apply wf_var with s1 ; auto with coc core arith datatypes.
+
+rewrite <- distr_lift_subst.
+apply IHIHc2 ; auto with coc core arith datatypes.
+
+cut (wf (lift_rec 1 T n :: f)).
+intro.
+apply type_prod with s1; auto with coc core arith datatypes.
+apply wf_var with s1; auto with coc core arith datatypes.
+
+cut (wf (lift_rec 1 T n :: f)).
+intro.
+apply type_sum with s1; auto with coc core arith datatypes.
+apply wf_var with s1; auto with coc core arith datatypes.
+
+cut (wf (lift_rec 1 T n :: f)).
+intro.
+apply type_subset ; auto with coc core arith datatypes.
+apply wf_var with set; auto with coc core arith datatypes.
+
+apply type_pi1 with (lift_rec 1 V (S n)) ; auto with coc.
+
+rewrite distr_lift_subst.
+simpl.
+apply type_pi2 with (lift_rec 1 U n); auto with coc.
+
+cut (wf (lift_rec 1 U n :: f)).
+intro.
+rewrite distr_lift_subst.
+apply type_let_in with (lift_rec 1 U n) s1 s2 ; auto with coc core.
+apply wf_var with s1 ; auto with coc core.
+
+apply type_conv with (lift_rec 1 U n) s; auto with coc core arith datatypes.
+
+apply coerce_prod with s ; auto with coc.
+apply IHIHc4; auto with coc.
+apply wf_var with s.
+apply IHIHc1 ; auto with coc core.
+
+apply coerce_sum with s ; auto with coc.
+apply IHIHc4; auto with coc.
+apply wf_var with s.
+apply IHIHc2 ; auto with coc core.
+
+apply coerce_beta with (lift_rec 1 B n) (lift_rec 1 C n) s ; auto with coc core.
 Qed.
 
 
@@ -84,6 +187,16 @@ unfold lift in |- *.
 intros.
 inversion_clear H0.
 apply typ_weak_weak with A e; auto with coc core arith datatypes.
+apply wf_var with s; auto with coc core arith datatypes.
+Qed.
+
+Theorem thinning_coerce : 
+   forall e T U,
+   e |- T >> U -> 
+   forall A, wf (A :: e) -> (A :: e) |- (lift 1 T) >> (lift 1 U).
+unfold lift ; intros.
+inversion_clear H0.
+apply coerce_weak_weak with A e; auto with coc core arith datatypes.
 apply wf_var with s; auto with coc core arith datatypes.
 Qed.
 
@@ -112,3 +225,69 @@ apply typ_wf with x (Srt s); auto with coc core arith datatypes.
 
 apply wf_var with s; auto with coc core arith datatypes.
 Qed.
+
+  Lemma thinning_n_coerce :
+   forall n e f,
+   trunc _ n e f ->
+   forall T U, f |- T >> U -> wf e -> e |- (lift n T) >> (lift n U).
+simple induction n.
+intros.
+rewrite lift0.
+rewrite lift0.
+replace e with f; auto with coc core arith datatypes.
+inversion_clear H; auto with coc core arith datatypes.
+
+do 8 intro.
+inversion_clear H0.
+intro.
+rewrite simpl_lift; auto with coc core arith datatypes.
+pattern (lift (S n0) T) in |- *.
+rewrite simpl_lift; auto with coc core arith datatypes.
+inversion_clear H0.
+replace (lift (S n0) U) with (lift 1 (lift n0 U)).
+apply thinning_coerce; auto with coc core arith datatypes.
+apply H with f; auto with coc core arith datatypes.
+apply typ_wf with x (Srt s); auto with coc core arith datatypes.
+
+apply wf_var with s; auto with coc core arith datatypes.
+rewrite <- simpl_lift.
+auto.
+Qed.
+
+Lemma wf_sort_lift :
+ forall n e t, wf e -> item_lift t e n -> exists s : sort, typ e t (Srt s).
+simple induction n.
+simple destruct e; intros.
+elim H0; intros.
+inversion_clear H2.
+
+elim H0; intros.
+rewrite H1.
+inversion_clear H2.
+inversion_clear H.
+exists s.
+replace (Srt s) with (lift 1 (Srt s)); auto with coc core arith datatypes.
+apply thinning; auto with coc core arith datatypes.
+apply wf_var with s; auto with coc core arith datatypes.
+
+intros.
+elim H1; intros.
+rewrite H2.
+generalize H0.
+inversion_clear H3; intros.
+rewrite simpl_lift; auto with coc core arith datatypes.
+cut (wf l); intros.
+elim H with l (lift (S n0) x); intros; auto with coc core arith datatypes.
+inversion_clear H3.
+exists x0.
+change (typ (y :: l) (lift 1 (lift (S n0) x)) (lift 1 (Srt x0))) in |- *.
+apply thinning; auto with coc core arith datatypes.
+apply wf_var with s; auto with coc core arith datatypes.
+
+exists x; auto with coc core arith datatypes.
+
+inversion_clear H3.
+apply typ_wf with y (Srt s); auto with coc core arith datatypes.
+Qed.
+
+Hint Resolve thinning_n thinning_n_coerce : coc.
